Extend the flag to have values: NoActions, OnlyGetTrace, IOActions, AllActions

io/IIO2.fst
@@ -4,60 +4,77 @@ open FStar.Tactics
 open ExtraTactics
 open FStar.Calc
 
-open Common
 open DMFree
 open IO.Sig
 open IO.Sig.Call
 open IO
 open IIO
 
-let rec contains (m:iio 'a) =
-match m with
-| Return x -> False
-| Call GetTrace _ _ -> True 
-| Call cmd arg k -> forall r. contains (k r)
-| PartialCall pre k -> forall r. contains (k r)
-
 (** fstar does not like type bool as an index for an effect --- not sure why **)
 noeq
-type tflag = | Contains | NotContain
+type tflag = | NoActions | OnlyGetTrace | IOActions | AllActions
+
+let rec satisfies (m:iio 'a) (flag:tflag) =
+match flag, m with
+| AllActions,   _                     -> True
+| _,            Return x              -> True
+| _,            PartialCall pre k     -> forall r. satisfies (k r) flag
+| NoActions,    _                     -> False
+| OnlyGetTrace, Call GetTrace arg k   -> forall r. satisfies (k r) flag
+| OnlyGetTrace, Call cmd arg k        -> False
+| IOActions,    Call GetTrace arg k   -> False
+| IOActions,    Call cmd arg k        -> forall r. satisfies (k r) flag
+
 let (+) (flag1:tflag) (flag2:tflag) = 
   match flag1, flag2 with
-  | NotContain, NotContain -> NotContain
-  | _ -> Contains
+  | NoActions, NoActions -> NoActions
+  | NoActions, fl -> fl
+  | fl, NoActions -> fl
+  | OnlyGetTrace, OnlyGetTrace -> OnlyGetTrace
+  | IOActions, IOActions -> IOActions
+  | _, _ -> AllActions
 
 let (<=) (flag1:tflag) (flag2:tflag) =
   match flag1, flag2 with
-  | Contains, NotContain -> False
-  | _ -> True
+  | NoActions, _ -> True
+  | OnlyGetTrace, NoActions -> False
+  | OnlyGetTrace, _ -> True
+  | IOActions, NoActions -> False
+  | IOActions, OnlyGetTrace -> False
+  | IOActions, _ -> True
+  | AllActions, AllActions -> True
+  | AllActions, _ -> False
 
-type dm_gio (a:Type) (flag:tflag) (wp:hist a) = t:(dm_iio a wp){contains t ==> Contains? flag} 
+type dm_gio (a:Type) (flag:tflag) (wp:hist a) = t:(dm_iio a wp){t `satisfies` flag} 
   // if the tree contains GetTrace, then the flag must be true
 
 (** ** Model compilation **)
-assume type ct (m:Type->Type)
-assume type pt (m:Type->Type)
+assume type ct (m:Type u#a -> Type u#(max 1 a))
+assume type pt (m:Type u#a -> Type u#(max 1 a))
 
-let gio flag (a:Type) = dm_gio a flag trivial_hist
+type gio flag (a:Type u#a) : Type u#(max 1 a) = dm_gio a flag trivial_hist
 
 // This way prog_s can not use `GetTrace`.
 // even if prog_s whould check if `fl2` is true, the refinement on the tree is stronger
-type prog_s = #fl:tflag -> ct (gio fl) -> pt (gio fl)
+type prog_s = #fl:tflag -> ct (gio fl) -> pt (gio (fl + IOActions))
 // I suppose ctx_s can also be parametric in the flag, but not sure if needed
-type ctx_s = ct (gio NotContain)
-let link_s (p:prog_s) (c:ctx_s) = p #NotContain c
+type ctx_s = #fl:tflag -> ct u#a (gio fl)
+let link_s (p:prog_s) (c:ctx_s) = p #IOActions c
 
-type prog_t = ct (gio Contains) -> pt (gio Contains)
-type ctx_t  = m:(Type->Type) -> ct m 
-let link_t (p:prog_t) (c:ctx_t) = p (c (gio Contains))
+type prog_t = ct (gio AllActions) -> pt (gio AllActions)
+type ctx_t  = m:(Type u#a ->Type u#(max 1 a)) -> ct m 
+let link_t (p:prog_t) (c:ctx_t) = p (c (gio AllActions))
 
-let compile_p (p:prog_s) : prog_t = fun (c:ct (gio Contains)) -> p c
+let compile_p (p:prog_s) : prog_t = fun (c:ct (gio AllActions)) -> p c
+
+val backtranslate : ctx_t u#a -> ctx_s u#a
+let backtranslate c (#fl:tflag) = c (gio fl)
 
 (** ** Defining F* Effect **)
 
 let dm_gio_theta #a = theta #a #iio_cmds #iio_sig #event iio_wps
 
-let dm_gio_return (a:Type) (x:a) : dm_gio a NotContain (hist_return x) by (compute ()) =
+let dm_gio_return (a:Type) (x:a) : dm_gio a NoActions (hist_return x) by (compute ()) =
   dm_iio_return a x
 
 val dm_gio_bind  : 
@@ -72,10 +89,7 @@ val dm_gio_bind  :
   Tot (dm_gio b (flag_v + flag_f) (hist_bind wp_v wp_f))
 let dm_gio_bind a b flag_v flag_f wp_v wp_f v f : (dm_gio b (flag_v + flag_f) (hist_bind wp_v wp_f)) = 
   let r = dm_iio_bind a b wp_v wp_f v f in
-  assert (Contains? flag_v \/ Contains? flag_f ==> Contains? (flag_v + flag_f));
-  assert (NotContain? flag_v /\ NotContain? flag_f ==> 
-        (~(contains v) /\ (forall x. ~(contains (f x))))); // ==> ~(contains r));
-  assume (~(contains v) /\ (forall x. ~(contains (f x))) ==> ~(contains r));
+  assume (v `satisfies` flag_v /\ (forall x. f x `satisfies` flag_f) ==> r `satisfies` (flag_v + flag_f));
   r
 
 val dm_gio_subcomp : 
@@ -87,47 +101,81 @@ val dm_gio_subcomp :
   f: dm_gio a flag1 wp1 ->
   Pure (dm_gio a flag2 wp2) ((flag1 <= flag2) /\ hist_ord wp2 wp1) (fun _ -> True)
 let dm_gio_subcomp a flag1 flag2 wp1 wp2 f = 
+  admit ();
   dm_iio_subcomp a wp1 wp2 f
 
-let dm_gio_if_then_else a _ _ wp1 wp2 f g b = dm_if_then_else iio_cmds iio_sig event iio_wps a wp1 wp2 f g b
+let dm_gio_if_then_else (a : Type u#a) (fl1 fl2:tflag)
+  (wp1 wp2: hist a) (f : dm_gio a fl1 wp1) (g : dm_gio a fl2 wp2) (b : bool) : Type =
+  dm_gio a (fl1 + fl2) (hist_if_then_else wp1 wp2 b)
 
 total
 reflectable
 effect {
-  GIOwp (a:Type) (flag:tflag) (wp : hist a) 
+  GIOwp (a:Type) (flag:tflag) (wp : hist #event a) 
   with {
        repr       = dm_gio
      ; return     = dm_gio_return
      ; bind       = dm_gio_bind 
      ; subcomp    = dm_gio_subcomp
- //    ; if_then_else = dm_gio_if_then_else
+     ; if_then_else = dm_gio_if_then_else
      }
 }
 
-let lift_io_gio (a:Type) (wp:hist a) (f:dm_io a wp) :
-  Tot (dm_gio a NotContain wp) =
-  admit ();
-  lift_io_iio a wp f
-  
-sub_effect IOwp ~> GIOwp = lift_io_gio
+let dm_gio_partial_return 
+  (pre:pure_pre) : dm_gio (squash pre) NoActions (partial_call_wp pre) by (compute ()) =
+  dm_partial_return iio_cmds iio_sig event iio_wps pre
 
-let get_trace () : GIOwp trace Contains
+val lift_pure_dm_gio :
+  a: Type ->
+  w: pure_wp a ->
+  f: (eqtype_as_type unit -> PURE a w) ->
+  Tot (dm_gio a NoActions (wp_lift_pure_hist w))
+let lift_pure_dm_gio a w f = 
+  lemma_wp_lift_pure_hist_implies_as_requires #a #event w;
+  FStar.Monotonic.Pure.elim_pure_wp_monotonicity_forall ();
+  let lhs : dm_gio _ NoActions _ = dm_gio_partial_return (as_requires w) in
+  let rhs = (fun (pre:(squash (as_requires w))) -> dm_gio_return a (f pre)) in
+  let m = dm_gio_bind _ _ NoActions NoActions _ _ lhs rhs in
+  dm_gio_subcomp a NoActions NoActions _ _ m
+  
+sub_effect PURE ~> GIOwp = lift_pure_dm_gio
+
+effect GIO
+  (a:Type)
+  (fl:tflag)
+  (pre : trace -> Type0)
+  (post : trace -> a -> trace -> Type0) =
+  GIOwp a fl (to_hist pre post) 
+  
+let static_cmd
+  (cmd : io_cmds)
+  (arg : io_sig.args cmd) :
+  GIO (io_resm cmd) IOActions
+    (requires (fun h -> io_pre cmd arg h))
+    (ensures (fun h (r:io_sig.res cmd arg) lt ->
+        lt == [convert_call_to_event cmd arg r])) =
+  GIOwp?.reflect (iio_call cmd arg)
+
+let get_trace () : GIOwp trace OnlyGetTrace
   (fun p h -> forall lt. lt == [] ==> p lt h) =
   GIOwp?.reflect (iio_call GetTrace ())
 
-let prog (#fl:tflag) (c:unit -> GIOwp unit fl trivial_hist) : GIOwp unit fl trivial_hist =
-  (**
-  if Contains? fl then
-    let h = get_trace () in // not possible because it does not know if fl2 is true or not
-    ()
-  else **)
-  c ()
+open FStar.Ghost
 
-let ctx (_:unit) : GIOwp unit NotContain trivial_hist = ()
+let bady (_:unit) : GIOwp unit OnlyGetTrace trivial_hist = ()
 
-let test2 () : GIOwp unit Contains trivial_hist = prog #NotContain ctx
+let prog (#fl:tflag) (c:unit -> GIOwp unit fl trivial_hist) : GIOwp unit fl trivial_hist 
+// by (explode (); bump_nth 7; dump "H") 
+ =
+  match fl with
+//  | AllActions -> bady ()
+  | _ -> c ()
 
-let performance_test (#fl:tflag) : GIOwp unit fl (fun p h -> forall lt. (List.length lt == 6) \/ (List.length lt == 7) ==> p lt ()) =
+let ctx (_:unit) : GIOwp unit NoActions trivial_hist = ()
+
+let test2 () : GIOwp unit AllActions trivial_hist = prog #AllActions ctx
+
+let performance_test (#fl:tflag) : GIOwp unit (fl+IOActions) (fun p h -> forall lt. (List.length lt == 6) \/ (List.length lt == 7) ==> p lt ()) =
   let fd = static_cmd Openfile "../Makefile" in
   let fd = static_cmd Openfile "../Makefile" in
   let fd = static_cmd Openfile "../Makefile" in
